ver3_less_complex/common/proofs.dfy
@@ -1,5 +1,10 @@
+// include "sets.dfy"
+include "../Auxilarily.dfy"
 module M_ProofTactic
 {
+    import opened M_Set
+    import opened M_AuxilarilyFunc
+
     lemma LemmaSubsetTransitiveInSeq<T> (s : seq<set<T>>)
     requires |s| > 0
     requires forall i | 0 <= i < |s|-1 :: s[i] <= s[i+1]
@@ -17,4 +22,57 @@ module M_ProofTactic
         }
     }
 
+    lemma LemmaSetEqualityTransitiveInSeq<T> (s : seq<set<T>>)
+    requires |s| > 0
+    requires forall i | 0 <= i < |s|-1 :: s[i] == s[i+1]
+    ensures forall i | 0 <= i <= |s|-1 :: s[0] == s[i]
+    ensures forall i, j | && 0 <= i <= |s|-1
+                          && 0 <= j <= |s|-1
+                        ::
+                          s[i] == s[j]
+    {
+        forall i | 0 <= i <= |s|-1
+        ensures s[0] == s[i] {
+            if |s| == 1 {
+            }
+            else
+            {
+                LemmaSetEqualityTransitiveInSeq(s[1..]);
+            }
+        }
+    }
+
+    lemma LemmaSeqCumulative<T> (a : seq<set<T>>, b : seq<set<T>>)
+    requires |b| > 0
+    requires |a| == |b| + 1
+    requires forall i | 0 < i < |a| :: a[i] == a[i-1] + b[i-1]
+    ensures a[|a|-1] == a[0] + setUnionOnSeq(b)
+    {
+        if |b| == 1
+        {
+        }
+        else 
+        {
+            LemmaSeqCumulative(a[1..], b[1..]);
+        }
+    }
+
+    predicate prepareImp1<T> (outMsg : set<T>)
+    {
+        forall vote | vote in outMsg ::
+                                && outMsg == {vote}
+    }
+
+    predicate prepareImp2<T> (outMsg : set<T>)
+    {
+        var votes := outMsg;
+        outMsg == votes
+    }
+
+    lemma LemmaRefactorTest<T> (outMsg : set<T>)
+    requires prepareImp1(outMsg)
+    ensures prepareImp2(outMsg)
+    {
+        // assert |outMsg| <= 1;
+    }
 }
