ver3_less_complex/Axioms.dfy
@@ -11,4 +11,7 @@ module M_Axiom {
     lemma{:axiom} Axiom_Byz_Constraints()
     ensures |Adversary_Nodes| <= f(|All_Nodes|)
     ensures Adversary_Nodes * Honest_Nodes == {}
+
+    lemma{:axiom} NoOuterClient()
+    ensures forall id : Address :: id in All_Nodes
 }
