ver3_less_complex/Lemma_Test.dfy
@@ -1,0 +1,34 @@
+include "Type.dfy"
+include "Auxilarily.dfy"
+include "Replica.dfy"
+
+module M_Lemma_Test {
+    import opened M_SpecTypes
+    import opened M_Replica
+    import opened M_AuxilarilyFunc
+
+
+    lemma LemmaPreparePhaseSendOutPrepareVote(r : ReplicaState,
+                                              r' : ReplicaState,
+                                              outMsg : set<Msg>)
+    requires ValidReplicaState(r)
+    requires UponPrepare(r, r', outMsg)
+    ensures forall vote | vote in outMsg
+                        :: 
+                          vote.partialSig.Signature?
+                          ==>
+                          vote.partialSig.mType.MT_Prepare?
+    {
+    }
+
+    lemma LemmaValidMsgTest(m : Msg, id : nat)
+    requires id > 0
+    requires ValidMsg(m)
+    ensures m.mType.MT_NewView? ==> ValidQC(m.justify) && m.justify.cType.MT_Prepare?
+    {
+        if m.mType.MT_NewView? && ValidQC(m.justify) {
+            assert m.viewNum != id - 1;
+        }
+    }
+
+}
