ver3_less_complex/Lemmas.dfy
@@ -3,6 +3,8 @@ include "Auxilarily.dfy"
 include "System.dfy"
 include "Trace.dfy"
 include "Replica.dfy"
+include "Axioms.dfy"
+include "common/sets.dfy"
 
 module M_Lemma {
     import opened M_SpecTypes
@@ -10,22 +12,31 @@ module M_Lemma {
     import opened M_System
     import opened M_Trace
     import opened M_Replica
-
-    lemma{:axiom} NoOuterClient()
-    ensures forall cert : Signature :: cert.Signature? ==> cert.signer in All_Nodes
+    import opened M_Axiom
+    import opened M_Set
 
     /*>>>>>>>>>>>>>>>>>>>>>>> START : Lemmas For Message Transmisson  */
 
+    /* If an honest replica send out a vote message,
+       then this message should be found in its output buffer (msgSent).
+       The reason we can conclude this is that we assume signatures cannot
+       be forged by byzantine nodes 
+       TODO: It would be more rational if we make a new axiom to describe
+             signatures cannot be forged, and use it to prove this lemma.
+       */
     lemma LemmaExistVoteMsgForSignature(ss : SystemState)
     requires Reachable(ss)
     ensures forall sig : Signature |  && sig.Signature?
                                       && sig.signer in ss.nodeStates.Keys
                                       && IsHonest(ss, sig.signer)
                                    :: exists m | m in ss.nodeStates[sig.signer].msgSent
-                                              :: corrVoteMsg(sig, m)
+                                              :: 
+                                                && ValidVoteMsg(m)
+                                                && corrVoteMsg(sig, m)
                                                  
 
     /*<<<<<<<<<<<<<<<<<<<<<<< END : Lemmas For Message Transmisson */
+
 
     lemma LemmaExistVoteMsgIfCertificateFormed(ss : SystemState)
     requires Reachable(ss)
@@ -89,11 +100,31 @@ module M_Lemma {
                              && (exists m2 : Msg :: && m2 in ss.msgSent
                                                  && ValidQC(m2.justify)
                                                  && m2.justify.cType == MT_Prepare
-                                                 && m2.justify.block == m.justify.block
-                                                 && m2.justify.viewNum == m.justify.viewNum
+                                                 && correspondingQC(m.justify, m2.justify)
                             )
     {
-
+        forall m : Msg | && m in ss.msgSent
+                                && ValidQC(m.justify)
+                                && m.justify.cType == MT_PreCommit
+        ensures (exists m2 : Msg :: && m2 in ss.msgSent
+                                    && ValidQC(m2.justify)
+                                    && m2.justify.cType == MT_Prepare
+                                    && correspondingQC(m.justify, m2.justify)
+                            )
+        {
+            var sgns := m.justify.signatures;
+            var signers := set sig | sig in sgns :: sig.signer;
+            LemmaExistHonestSignerInValidQC(ss, m.justify);
+            LemmaReachableStateIsValid(ss);
+            var sign_honest :| && sign_honest in sgns
+                              && IsHonest(ss, sign_honest.signer);
+            LemmaExistVoteMsgForSignature(ss);
+            var corrVote :| && corrVote in ss.nodeStates[sign_honest.signer].msgSent
+                            && ValidVoteMsg(corrVote)
+                            && corrVoteMsg(sign_honest, corrVote);
+            assert ValidPrecommitVote(corrVote);
+            HonestReplicaVotePrecommitOnlyWhenItReceivePrepareQC(ss, sign_honest.signer);
+        }
     }
 
     lemma LemmaExistValidPrecommitQCForEveryValidCommitQC(ss : SystemState)
@@ -108,7 +139,28 @@ module M_Lemma {
                                                     && correspondingQC(m.justify, m2.justify)
                             )
     {
-
+        forall m : Msg | && m in ss.msgSent
+                                && ValidQC(m.justify)
+                                && m.justify.cType == MT_Commit
+        ensures (exists m2 : Msg :: && m2 in ss.msgSent
+                                    && ValidQC(m2.justify)
+                                    && m2.justify.cType == MT_PreCommit
+                                    && correspondingQC(m.justify, m2.justify)
+                            )
+        {
+            var sgns := m.justify.signatures;
+            var signers := set sig | sig in sgns :: sig.signer;
+            LemmaExistHonestSignerInValidQC(ss, m.justify);
+            LemmaReachableStateIsValid(ss);
+            var sign_honest :| && sign_honest in sgns
+                              && IsHonest(ss, sign_honest.signer);
+            LemmaExistVoteMsgForSignature(ss);
+            var corrVote :| && corrVote in ss.nodeStates[sign_honest.signer].msgSent
+                            && ValidVoteMsg(corrVote)
+                            && corrVoteMsg(sign_honest, corrVote);
+            assert ValidCommitVote(corrVote);
+            HonestReplicaVoteCommitOnlyWhenItReceivePrecommitQC(ss, sign_honest.signer);
+        }
     }
 
 
@@ -126,19 +178,6 @@ module M_Lemma {
         LemmaExistValidPrecommitQCForEveryValidCommitQC(ss);
         LemmaExistValidPrepareQCForEveryValidPrecommitQC(ss);
     }
-
-    // lemma LemmaPrepareQCWithLowerViewIsExtensionOfPrepareQCWithHigherView(ss : SystemState)
-    // requires Reachable(ss)
-    // ensures forall m1, m2 : Msg | && m1 in ss.msgSent
-    //                               && m2 in ss.msgSent
-    //                               && msgWithValidQC(m1, MT_Prepare)
-    //                               && msgWithValidQC(m2, MT_Prepare)
-    //                               && m1.justify.viewNum <= m2.justify.viewNum
-    //                             ::
-    //                               extension(m1.justify.block, m2.justify.block)
-    // {
-    //     LemmaPrepareQCExtensionIfExistCommitQC(ss);
-    // }
     
     lemma LemmaPrepareQCExtensionIfExistCommitQC(ss : SystemState)
     requires Reachable(ss)
@@ -159,31 +198,31 @@ module M_Lemma {
                             )
                          :: 
                             extension(m2.justify.block, m1.justify.block)
-    // {
-    //     if SystemInit(ss) {
-    //         // assert ss.msgSent == {};
-    //     }
-    //     else {
-    //         forall m1, m2 | && m1 in ss.msgSent
-    //                         && m2 in ss.msgSent
-    //                         && msgWithValidQC(m1, MT_Prepare)
-    //                         && msgWithValidQC(m2, MT_Prepare)
-    //                         && m1.justify.viewNum <= m2.justify.viewNum
-    //                         && (
-    //                             exists m1_commit, m2_commit |
-    //                                                           && m1_commit in ss.msgSent
-    //                                                           && m2_commit in ss.msgSent
-    //                                                           && msgWithValidQC(m1_commit, MT_Commit)
-    //                                                           && msgWithValidQC(m2_commit, MT_Commit)
-    //                                                         ::
-    //                                                           && correspondingQC(m1.justify, m1_commit.justify)
-    //                                                           && correspondingQC(m2.justify, m2_commit.justify)
-    //                         )
-    //         ensures extension(m2.justify.block, m1.justify.block)
-    //         {
-    //         }
-    //     }
-    // }
+    {
+        // if SystemInit(ss) {
+        //     // assert ss.msgSent == {};
+        // }
+        // else {
+        //     forall m1, m2 | && m1 in ss.msgSent
+        //                     && m2 in ss.msgSent
+        //                     && msgWithValidQC(m1, MT_Prepare)
+        //                     && msgWithValidQC(m2, MT_Prepare)
+        //                     && m1.justify.viewNum <= m2.justify.viewNum
+        //                     && (
+        //                         exists m1_commit, m2_commit |
+        //                                                       && m1_commit in ss.msgSent
+        //                                                       && m2_commit in ss.msgSent
+        //                                                       && msgWithValidQC(m1_commit, MT_Commit)
+        //                                                       && msgWithValidQC(m2_commit, MT_Commit)
+        //                                                     ::
+        //                                                       && correspondingQC(m1.justify, m1_commit.justify)
+        //                                                       && correspondingQC(m2.justify, m2_commit.justify)
+        //                     )
+        //     ensures extension(m2.justify.block, m1.justify.block)
+        //     {
+        //     }
+        // }
+    }
 
 
     lemma LemmaReachableStateIsValid(ss : SystemState)
@@ -201,6 +240,13 @@ module M_Lemma {
                                                            && SystemNext(run[i], run[i+1]));
             forall i | 0 < i <= |run|-1
             ensures ValidSystemState(run[i]) {
+                // if run[i-1] == run[i] {}
+                // else {
+                //     assert (exists replica, msgReceivedByNodes, msgSentByNodes
+                //                     | msgReceivedByNodes <= run[i-1].msgSent
+                //                     :: SystemNextByOneReplica(run[i-1], run[i], replica, msgReceivedByNodes, msgSentByNodes));
+                //     LemmaSystemTransitionHoldsValidity(run[i-1], run[i]);
+                // }
                 LemmaSystemTransitionHoldsValidity(run[i-1], run[i]);
             }
         } else {
@@ -226,7 +272,36 @@ module M_Lemma {
 
     }
 
+    lemma HonestReplicaVoteCommitOnlyWhenItReceivePrecommitQC(ss : SystemState, r : Address)
+    requires Reachable(ss)
+    requires IsHonest(ss, r)
+    ensures forall m | && m in ss.nodeStates[r].msgSent
+                       && ValidCommitVote(m)
+                    :: 
+                    //    && m.partialSig.mType.MT_Commit?
+                    //    && m.partialSig.Signature?
+                    //    ==>
+                       exists m2 | m2 in ss.nodeStates[r].msgReceived
+                                ::
+                                   && ValidCommitRequest(m2)
+                                   && corrVoteMsgAndToVotedMsg(m, m2)
+    {
+        LemmaReachableStateIsValid(ss);
+    }
 
+    lemma HonestReplicaVotePrecommitOnlyWhenItReceivePrepareQC(ss : SystemState, r : Address)
+    requires Reachable(ss)
+    requires IsHonest(ss, r)
+    ensures forall m | && m in ss.nodeStates[r].msgSent
+                       && ValidPrecommitVote(m)
+                    :: 
+                       exists m2 | m2 in ss.nodeStates[r].msgReceived
+                                ::
+                                   && ValidPrecommitRequest(m2)
+                                   && corrVoteMsgAndToVotedMsg(m, m2)
+    {
+        LemmaReachableStateIsValid(ss);
+    }
 
     lemma LemmaCommitQCVoteOnlyExistCorrespondingPrecommitQC(
         r : ReplicaState,
@@ -236,10 +311,9 @@ module M_Lemma {
     )
     requires ValidReplicaState(r)
     requires ReplicaNext(r, inMsg, r', outMsg)
-    ensures forall m | m in outMsg
-                    :: && m.partialSig.Signature?
-                       && m.mType.MT_Commit?
-                       ==>
+    ensures forall m | && m in outMsg
+                       && ValidCommitVote(m)
+                    :: 
                        exists m2 | m2 in r'.msgReceived
                                 :: 
                                    && ValidQC(m2.justify)
@@ -248,18 +322,17 @@ module M_Lemma {
                                    && m2.justify.viewNum == m.partialSig.viewNum
     {
         forall m | && m in outMsg
-                   && m.partialSig.Signature?
-                   && m.mType.MT_Commit?
+                   && ValidCommitVote(m)
         ensures exists m2 | m2 in r'.msgReceived
-                                :: 
-                                   && ValidQC(m2.justify)
-                                   && m2.justify.cType.MT_PreCommit?
-                                   && m2.justify.block == m.partialSig.block
-                                   && m2.justify.viewNum == m.partialSig.viewNum
+                         :: 
+                            && ValidQC(m2.justify)
+                            && m2.justify.cType.MT_PreCommit?
+                            && m2.justify.block == m.partialSig.block
+                            && m2.justify.viewNum == m.partialSig.viewNum
         {
-            var allMsgReceived := r.msgReceived + inMsg;
+            // var allMsgReceived := r.msgReceived + inMsg;
             var replicaWithNewMsgReceived := r.(
-                msgReceived := allMsgReceived
+                msgReceived := r.msgReceived + inMsg
             );
             var s : seq<ReplicaState>, o : seq<set<Msg>> :|
                 && |s| > 2
@@ -271,12 +344,59 @@ module M_Lemma {
                     && ReplicaNextSubStep(s[i], s[i+1], o[i])
                 )
                 && outMsg == setUnionOnSeq(o);
-            LemmaElementInSetUnionOnSeqMustExistInOneOfTheSets(m, o);
-            assert exists i | 0 <= i < |o| :: m in o[i];
+            assert exists i | 0 <= i < |o| :: m in o[i] by {
+                LemmaElementInSetUnionOnSeqMustExistInOneOfTheSets(m, o);
+            }
             var i :| 0 <= i < |o| && m in o[i];
-            assert UponPrepare(s[i], s[i+1], o[i]);
-            // LemmaMsgRelationInReplicaNext(r, inMsg, r', outMsg);
-            // assert UponCommit(r, r', outMsg);
+            assert  && UponCommit(s[i], s[i+1], o[i])
+                    && (exists m3 | m3 in r'.msgReceived
+                                :: 
+                                && ValidQC(m3.justify)
+                                && m3.justify.cType.MT_PreCommit?
+                                && m3.justify.block == m.partialSig.block
+                                && m3.justify.viewNum == m.partialSig.viewNum) by {
+                assert ValidReplicaState(s[i]);
+                assert ReplicaNextSubStep(s[i], s[i+1], o[i]);
+                LemmaReplicaVoteCommitOnlyWhenReceiveValidPrecommitQC(s[i], s[i+1], o[i]);
+                assert r'.msgReceived == s[i+1].msgReceived by {
+                    assert r' == s[|s|-1];
+                    LemmaReplicaMsgReceiveStableInNextSubSeq(s, o);
+                }
+            }
+            
         }
     }
+
+    /**
+        Lemmas for Quorum Certificate
+     */
+    lemma LemmaExistHonestSignerInValidQC(ss : SystemState, qc : Cert)
+    requires Reachable(ss)
+    requires ValidQC(qc)
+    ensures exists sig | sig in qc.signatures
+                       ::
+                         IsHonest(ss, sig.signer)
+    {
+        var sgns := qc.signatures;
+        assert |sgns| >= quorum(|M_SpecTypes.All_Nodes|);
+        var signers := set sig | sig in sgns :: sig.signer;
+        NumVoters(sgns);
+        assert |signers| >= quorum(|M_SpecTypes.All_Nodes|);
+        Axiom_Common_Constraints();
+        Axiom_Byz_Constraints();
+        LemmaHonestInQuorum(M_SpecTypes.All_Nodes,
+                            M_SpecTypes.Adversary_Nodes,
+                            signers);
+        var honest :| && honest in signers
+                      && honest in M_SpecTypes.Honest_Nodes;
+        assert All_Nodes == Honest_Nodes + Adversary_Nodes;
+        assert Honest_Nodes * Adversary_Nodes == {};
+        LemmaAdditiveOnSeparateSet(All_Nodes, Adversary_Nodes, Honest_Nodes);
+        assert Honest_Nodes == All_Nodes - Adversary_Nodes;
+        LemmaReachableStateIsValid(ss);
+        assert IsHonest(ss, honest);
+    }
+
+
+
 }
